running second mill version

examples/wysteria/mill2.fst
@@ -17,7 +17,12 @@ let ab = union alice_s bob_s
 type pre  (m:mode)  = fun m0 -> b2t (m0 = m)
 type post (#a:Type) = fun (m:mode) (x:a) -> True
 
-val mill2_sec: x:Box nat alice_s -> y:Box nat bob_s -> Wys bool (pre (Mode Par ab)) post
+val read_fn: unit -> Wys nat (fun m0 -> Mode.m m0 = Par /\
+                                        (exists p. Mode.ps m0 = singleton p))
+                             (fun m0 r -> True)
+let read_fn x = read #nat ()
+
+val mill2_sec: x:Box int alice_s -> y:Box int bob_s -> Wys bool (pre (Mode Par ab)) post
 let mill2_sec x y =
   let g:unit -> Wys bool (pre (Mode Sec ab)) post =
     fun _ -> (unbox_s x) > (unbox_s y)
@@ -26,10 +31,11 @@ let mill2_sec x y =
 
 val mill2: unit -> Wys bool (pre (Mode Par ab)) post
 let mill2 _ =
-  let x = as_par alice_s (read #nat) in
-  let y = as_par bob_s (read #nat) in
+  let x = as_par alice_s read_fn in
+  let y = as_par bob_s read_fn in
   mill2_sec x y
 
 ;;
 
-let _ = main ab mill2 in ()
+let x = main ab mill2 in
+wprint x
